rename for clarity, tidy

isabelle/CVM_Original/Utils/Utils_Basic.thy
@@ -72,41 +72,32 @@ lemma foldM_eq_foldM_enumerate :
 
 end
 
-definition find_last_before :: \<open>nat \<Rightarrow> 'a list \<Rightarrow> 'a \<Rightarrow> nat\<close> where
-  \<open>find_last_before \<equiv> \<lambda> k. last_index <<< take (Suc k)\<close>
+definition last_index_up_to :: \<open>nat \<Rightarrow> 'a list \<Rightarrow> 'a \<Rightarrow> nat\<close> where
+  \<open>last_index_up_to \<equiv> \<lambda> k. last_index <<< take (Suc k)\<close>
 
-lemma find_last_before_bound:
-  \<open>find_last_before n xs x \<le> Suc n\<close>
-proof (cases n)
-  case 0
-  then show ?thesis
-    unfolding find_last_before_def
-    by (metis One_nat_def last_index_less_size_conv last_index_size_conv length_take less_numeral_extra(4) less_or_eq_imp_le linorder_le_less_linear min_less_iff_conj)
-next
-  case (Suc n)
-  then show ?thesis
-    unfolding find_last_before_def
-    by (metis diff_self_eq_0 drop_eq_Nil2 drop_take dual_order.trans last_index_le_size take_eq_Nil2)
-qed
+lemma last_index_up_to_le :
+  \<open>last_index_up_to n xs x \<le> Suc n\<close>
+  unfolding last_index_up_to_def
+  by (metis cancel_comm_monoid_add_class.diff_cancel drop_eq_Nil drop_take dual_order.trans last_index_le_size take0)
 
 context
   fixes i xs
   assumes \<open>i < length xs\<close>
 begin
 
-lemma find_last_before_self_eq :
-  \<open>find_last_before i xs (xs ! i) = i\<close>
+lemma last_index_up_to_self_eq :
+  \<open>last_index_up_to i xs (xs ! i) = i\<close>
   using \<open>i < length xs\<close>
-  unfolding find_last_before_def
+  unfolding last_index_up_to_def
   by (simp add: take_Suc_conv_app_nth)
 
 lemma find_last_before_eq_find_last_iff :
   assumes \<open>x \<in> set (take i xs)\<close>
   shows
-    \<open>find_last_before i xs x = last_index (take i xs) x
+    \<open>last_index_up_to i xs x = last_index (take i xs) x
     \<longleftrightarrow> x \<noteq> xs ! i\<close>
   using assms \<open>i < length xs\<close>
-  unfolding find_last_before_def
+  unfolding last_index_up_to_def
   by (metis last_index_Snoc last_index_less_size_conv less_not_refl take_Suc_conv_app_nth)
 
 end
